redefine live paths

theory/Static_Communication_Analysis.thy
@@ -7,6 +7,7 @@ begin
 
 type_synonym label_map = "node_label \<Rightarrow> var set"
 
+
 inductive built_on_chan :: "abstract_value_env \<Rightarrow> label_map \<Rightarrow> var \<Rightarrow> var \<Rightarrow> bool"  where
   Chan: "
     \<lbrakk>
@@ -185,190 +186,6 @@ inductive static_chan_liveness :: "abstract_value_env \<Rightarrow> label_map \<
     static_chan_liveness V Ln Lx x\<^sub>c (LET x = APP f x\<^sub>a in e)
   "
 
-
-inductive is_static_live_flow :: "label_map \<Rightarrow> label_map \<Rightarrow> flow_set \<Rightarrow> flow_label \<Rightarrow> bool"  where
-  Next: "
-    (l, ENext, l') \<in> F \<Longrightarrow>
-    \<not> Set.is_empty (Lx l) \<Longrightarrow>
-    \<not> Set.is_empty (Ln l') \<Longrightarrow>
-    is_static_live_flow Ln Lx F (l, ENext, l')
-  " |
-  Spawn: "
-    (l, ENext, l') \<in> F \<Longrightarrow>
-    \<not> Set.is_empty (Lx l) \<Longrightarrow>
-    \<not> Set.is_empty (Ln l') \<Longrightarrow>
-    is_static_live_flow Ln Lx F (l, ESpawn, l')
-  " |
-  Call: "
-    (l, ENext, l') \<in> F \<Longrightarrow>
-    \<not> Set.is_empty (Lx l) \<Longrightarrow>
-    \<not> Set.is_empty (Ln l') \<Longrightarrow>
-    is_static_live_flow Ln Lx F (l, ECall, l')
-  " |
-  Return: "
-    (l, ENext, l') \<in> F \<Longrightarrow>
-    \<not> Set.is_empty (Lx l) \<Longrightarrow>
-    \<not> Set.is_empty (Ln l') \<Longrightarrow>
-    is_static_live_flow Ln Lx F (l, EReturn, l')
-  " |
-  Send: "
-    ((NLet xSend), ESend xM, (NLet xRecv)) \<in> F \<Longrightarrow>
-    {xM} \<subseteq> (Ln (NLet xSend)) \<Longrightarrow>
-    is_static_live_flow Ln Lx F ((NLet xSend), ESend xM, (NLet xRecv))
-  "
-
-inductive static_live_flow_graph :: "abstract_value_env \<Rightarrow> label_map \<Rightarrow> label_map \<Rightarrow> flow_set \<Rightarrow> exp \<Rightarrow> bool"  where
-  Result: "
-    static_live_flow_graph V Ln Lx F (RESULT x)
-  " |
-  Let_Unit: "
-    \<lbrakk>
-      static_live_flow_graph V Ln Lx F e;
-      Set.is_empty (Lx (NLet x)) \<or> Set.is_empty (Ln (nodeLabel e)) \<or>
-      {(NLet x , ENext, nodeLabel e)} \<subseteq> \<F>
-    \<rbrakk> \<Longrightarrow>
-    static_live_flow_graph V Ln Lx F (LET x = \<lparr>\<rparr> in e)
-  " |
-  Let_Chan: "
-    \<lbrakk>
-      static_live_flow_graph V Ln Lx F e;
-      Set.is_empty (Lx (NLet x)) \<or> Set.is_empty (Ln (nodeLabel e)) \<or>
-      {(NLet x , ENext, nodeLabel e)} \<subseteq> \<F>
-    \<rbrakk> \<Longrightarrow>
-    static_live_flow_graph V Ln Lx F (LET x = CHAN \<lparr>\<rparr> in e)
-  " |
-  Let_Send_Evt: "
-    \<lbrakk>
-      static_live_flow_graph V Ln Lx F e;
-      Set.is_empty (Lx (NLet x)) \<or> Set.is_empty (Ln (nodeLabel e)) \<or>
-      {(NLet x , ENext, nodeLabel e)} \<subseteq> \<F>
-    \<rbrakk> \<Longrightarrow>
-    static_live_flow_graph V Ln Lx F (LET x = SEND EVT x\<^sub>c x\<^sub>m in e)
-  " |
-  Let_Recv_Evt: "
-    \<lbrakk>
-      static_live_flow_graph V Ln Lx F e;
-      Set.is_empty (Lx (NLet x)) \<or> Set.is_empty (Ln (nodeLabel e)) \<or>
-      {(NLet x , ENext, nodeLabel e)} \<subseteq> \<F>
-    \<rbrakk> \<Longrightarrow>
-    static_live_flow_graph V Ln Lx F (LET x = RECV EVT x\<^sub>c in e)
-  " |
-  Let_Pair: "
-    \<lbrakk>
-      static_live_flow_graph V Ln Lx F e;
-      Set.is_empty (Lx (NLet x)) \<or> Set.is_empty (Ln (nodeLabel e)) \<or>
-      {(NLet x , ENext, nodeLabel e)} \<subseteq> \<F>
-    \<rbrakk> \<Longrightarrow>
-    static_live_flow_graph V Ln Lx F (LET x = \<lparr>x\<^sub>1, x\<^sub>2\<rparr> in e)
-  " |
-  Let_Left: "
-    \<lbrakk>
-      static_live_flow_graph V Ln Lx F e;
-      Set.is_empty (Lx (NLet x)) \<or> Set.is_empty (Ln (nodeLabel e)) \<or>
-      {(NLet x , ENext, nodeLabel e)} \<subseteq> \<F>
-    \<rbrakk> \<Longrightarrow>
-    static_live_flow_graph V Ln Lx F (LET x = LEFT x\<^sub>p in e)
-  " |
-  Let_Right: "
-    \<lbrakk>
-      static_live_flow_graph V Ln Lx F e;
-      Set.is_empty (Lx (NLet x)) \<or> Set.is_empty (Ln (nodeLabel e)) \<or>
-      {(NLet x , ENext, nodeLabel e)} \<subseteq> \<F>
-    \<rbrakk> \<Longrightarrow>
-    static_live_flow_graph V Ln Lx F (LET x = RIGHT x\<^sub>p in e)
-  " |
-  Let_Abs: "
-    \<lbrakk>
-      static_live_flow_graph V Ln Lx F e\<^sub>b;
-      static_live_flow_graph V Ln Lx F e;
-      Set.is_empty (Lx (NLet x)) \<or> Set.is_empty (Ln (nodeLabel e)) \<or>
-      {(NLet x , ENext, nodeLabel e)} \<subseteq> \<F>
-    \<rbrakk> \<Longrightarrow>
-    static_live_flow_graph V Ln Lx F (LET x = FN f x\<^sub>p . e\<^sub>b  in e)
-  " |
-  Let_Spawn: "
-    \<lbrakk>      
-      static_live_flow_graph V Ln Lx F e;
-      Set.is_empty (Lx (NLet x)) \<or> Set.is_empty (Ln (nodeLabel e)) \<or>
-      {(NLet x , ENext, nodeLabel e)} \<subseteq> \<F>;
-
-      static_live_flow_graph V Ln Lx F e\<^sub>c;
-      Set.is_empty (Lx (NLet x)) \<or> Set.is_empty (Ln (nodeLabel e\<^sub>c)) \<or>
-      {(NLet x, ESpawn, nodeLabel e\<^sub>c)} \<subseteq> \<F>
-
-    \<rbrakk> \<Longrightarrow>
-    static_live_flow_graph V Ln Lx F (LET x = SPAWN e\<^sub>c in e)
-  " |  
-  Let_Sync: "
-    \<lbrakk>
-      static_live_flow_graph V Ln Lx F e;
-      Set.is_empty (Lx (NLet x)) \<or> Set.is_empty (Ln (nodeLabel e)) \<or>
-      {(NLet x , ENext, nodeLabel e)} \<subseteq> \<F>;
-
-      (\<forall> xSC xM xC xRC y.
-        {xM} \<subseteq> (Ln (NLet x)) \<longrightarrow>
-        {^Send_Evt xSC xM} \<subseteq> V x\<^sub>e \<longrightarrow>
-        {^Chan xC} \<subseteq> V xSC \<longrightarrow>
-        {^Chan xC} \<subseteq> V xRC \<longrightarrow>
-        {^Recv_Evt xRC} \<subseteq> \<V> y \<longrightarrow>
-        {(NLet x, ESend xM, NLet y)} \<subseteq> \<F>
-      )
-    \<rbrakk> \<Longrightarrow>
-    static_live_flow_graph V Ln Lx F (LET x = SYNC x\<^sub>e in e)
-  " |
-  Let_Fst: "
-    \<lbrakk>
-      static_live_flow_graph V Ln Lx F e;
-      Set.is_empty (Lx (NLet x)) \<or> Set.is_empty (Ln (nodeLabel e)) \<or>
-      {(NLet x , ENext, nodeLabel e)} \<subseteq> \<F>
-    \<rbrakk> \<Longrightarrow>
-    static_live_flow_graph V Ln Lx F (LET x = FST x\<^sub>p in e)
-  " |
-  Let_Snd: "
-    \<lbrakk>
-      static_live_flow_graph V Ln Lx F e;
-      Set.is_empty (Lx (NLet x)) \<or> Set.is_empty (Ln (nodeLabel e)) \<or>
-      {(NLet x , ENext, nodeLabel e)} \<subseteq> \<F>
-    \<rbrakk> \<Longrightarrow>
-    static_live_flow_graph V Ln Lx F (LET x = SND x\<^sub>p in e)
-  " (* |
-  Let_Case: "
-    \<lbrakk>
-      {
-        (NLet x, ECall, nodeLabel e\<^sub>l),
-        (NLet x, ECall, nodeLabel e\<^sub>r),
-        (NResult (\<lfloor>e\<^sub>l\<rfloor>), EReturn, nodeLabel e),
-        (NResult (\<lfloor>e\<^sub>r\<rfloor>), EReturn, nodeLabel e)
-      } \<subseteq> \<F>;
-      static_live_flow_graph V Ln Lx F e\<^sub>l;
-      static_live_flow_graph V Ln Lx F e\<^sub>r;
-      static_live_flow_graph V Ln Lx F e
-    \<rbrakk> \<Longrightarrow>
-    static_live_flow_graph V Ln Lx F (LET x = CASE x\<^sub>s LEFT x\<^sub>l |> e\<^sub>l RIGHT x\<^sub>r |> e\<^sub>r in e)
-  " |
-  Let_App: "
-    \<lbrakk>
-      (\<forall> f' x\<^sub>p e\<^sub>b . ^Abs f' x\<^sub>p e\<^sub>b \<in> \<V> f \<longrightarrow>
-        {
-          (NLet x, ECall, nodeLabel e\<^sub>b),
-          (NResult (\<lfloor>e\<^sub>b\<rfloor>), EReturn, nodeLabel e)
-        } \<subseteq> \<F>);
-      static_live_flow_graph V Ln Lx F e
-    \<rbrakk> \<Longrightarrow>
-    static_live_flow_graph V Ln Lx F (LET x = APP f x\<^sub>a in e)
-  "
-*)
-
-inductive static_live_flow_set :: "label_map \<Rightarrow> label_map \<Rightarrow> flow_set \<Rightarrow> flow_set \<Rightarrow> bool"  where
-  "
-    (\<forall> l cl l' .
-      is_static_live_flow Ln Lx F (l, cl, l') \<longrightarrow>
-      (l, cl, l') \<in> LF 
-    ) \<Longrightarrow>
-    static_live_flow_set Ln Lx F LF
-  "
-
-
 inductive is_static_send_node_label :: "abstract_value_env \<Rightarrow> exp \<Rightarrow> var \<Rightarrow> node_label \<Rightarrow> bool" where
   Sync: "
     {^Chan xC} \<subseteq> V xSC \<Longrightarrow>
@@ -386,20 +203,36 @@ inductive is_static_recv_node_label :: "abstract_value_env \<Rightarrow> exp \<R
   "
 
 
-inductive is_static_path :: "flow_set \<Rightarrow> node_label \<Rightarrow> (node_label \<Rightarrow> bool) \<Rightarrow> static_path \<Rightarrow> bool" where
+inductive is_static_path :: "abstract_value_env \<Rightarrow> flow_set \<Rightarrow> label_map \<Rightarrow> var \<Rightarrow> node_label \<Rightarrow> (node_label \<Rightarrow> bool) \<Rightarrow> static_path \<Rightarrow> bool" where
   Empty: "
     isEnd start \<Longrightarrow>
-    is_static_path F start isEnd []
+    is_static_path V F Ln xC start isEnd []
   " |
   Edge: "
     isEnd end \<Longrightarrow>
     (start, edge, end) \<in> F \<Longrightarrow>
-    is_static_path F start isEnd [(start, el)]
+    is_static_path V F Ln xC start isEnd [(start, el)]
   " |
-  Step: "
-    is_static_path F middle isEnd ((middle, edge') # path) \<Longrightarrow>
-    (start, edge, middle) \<in> F \<Longrightarrow>
-    is_static_path F start isEnd ((start, edge) # (middle, edge') # path)
+  Step_Next: "
+    is_static_path V F Ln xC middle isEnd ((middle, edge') # path) \<Longrightarrow>
+    (start, ENext, middle) \<in> F \<Longrightarrow>
+    is_static_path V F Ln xC start isEnd ((start, edge) # (middle, edge') # path)
+  " |
+  Step_Call: "
+    is_static_path V F Ln xC middle isEnd ((middle, edge') # path) \<Longrightarrow>
+    (start, ECall, middle) \<in> F \<Longrightarrow>
+    is_static_path V F Ln xC start isEnd ((start, edge) # (middle, edge') # path)
+  " |
+  Step_Return: "
+    is_static_path V F Ln xC middle isEnd ((middle, edge') # path) \<Longrightarrow>
+    (start, EReturn, middle) \<in> F \<Longrightarrow>
+    is_static_path V F Ln xC start isEnd ((start, edge) # (middle, edge') # path)
+  " |
+  Step_Send: "
+    is_static_path V F Ln xC middle isEnd ((middle, edge') # path) \<Longrightarrow>
+    built_on_chan V Ln xC xM \<Longrightarrow>
+    (start, ESend xM, middle) \<in> F \<Longrightarrow>
+    is_static_path V F Ln xC start isEnd ((start, edge) # (middle, edge') # path)
   "
 
 
@@ -461,37 +294,33 @@ definition every_two_static_paths  :: "(static_path \<Rightarrow> bool) \<Righta
 
 inductive static_one_shot :: "abstract_value_env \<Rightarrow> exp \<Rightarrow> var \<Rightarrow> bool" where
   Sync: "
-    every_two_static_paths (is_static_path LF (NLet xC) (is_static_send_node_label V e xC)) singular \<Longrightarrow>
-    static_live_flow_set Ln Lx F LF \<Longrightarrow>
-    static_chan_liveness V Ln Lx Lo xC e \<Longrightarrow>
+    every_two_static_paths (is_static_path V F Ln xC (NLet xC) (is_static_send_node_label V e xC)) singular \<Longrightarrow>
+    static_chan_liveness V Ln Lx xC e \<Longrightarrow>
     static_flow_set V F e \<Longrightarrow>
     static_one_shot V e xC 
   "
 
 inductive static_one_to_one :: "abstract_value_env \<Rightarrow> exp \<Rightarrow> var \<Rightarrow> bool" where
   Sync: "
-    every_two_static_paths (is_static_path LF (NLet xC) (is_static_send_node_label V e xC)) noncompetitive \<Longrightarrow>
-    every_two_static_paths (is_static_path LF (NLet xC) (is_static_recv_node_label V e xC)) noncompetitive \<Longrightarrow>
-    static_live_flow_set Ln Lx F LF \<Longrightarrow>
-    static_chan_liveness V Ln Lx Lo xC e \<Longrightarrow>
+    every_two_static_paths (is_static_path V F Ln xC (NLet xC) (is_static_send_node_label V e xC)) noncompetitive \<Longrightarrow>
+    every_two_static_paths (is_static_path V F Ln xC (NLet xC) (is_static_recv_node_label V e xC)) noncompetitive \<Longrightarrow>
+    static_chan_liveness V Ln Lx xC e \<Longrightarrow>
     static_flow_set V F e \<Longrightarrow>
     static_one_to_one V e xC 
   "
 
 inductive static_fan_out :: "abstract_value_env \<Rightarrow> exp \<Rightarrow> var \<Rightarrow> bool" where
   Sync: "
-    every_two_static_paths (is_static_path LF (NLet xC) (is_static_send_node_label V e xC)) noncompetitive \<Longrightarrow>
-    static_live_flow_set Ln Lx F LF \<Longrightarrow>
-    static_chan_liveness V Ln Lx Lo xC e \<Longrightarrow>
+    every_two_static_paths (is_static_path V F Ln xC (NLet xC) (is_static_send_node_label V e xC)) noncompetitive \<Longrightarrow>
+    static_chan_liveness V Ln Lx xC e \<Longrightarrow>
     static_flow_set V F e \<Longrightarrow>
     static_fan_out V e xC 
   "
 
 inductive static_fan_in :: "abstract_value_env \<Rightarrow> exp \<Rightarrow> var \<Rightarrow> bool" where
   Sync: "
-    every_two_static_paths (is_static_path LF (NLet xC) (is_static_recv_node_label V e xC)) noncompetitive \<Longrightarrow>
-    static_live_flow_set Ln Lx F LF \<Longrightarrow>
-    static_chan_liveness V Ln Lx Lo xC e \<Longrightarrow>
+    every_two_static_paths (is_static_path V F Ln xC (NLet xC) (is_static_recv_node_label V e xC)) noncompetitive \<Longrightarrow>
+    static_chan_liveness V Ln Lx xC e \<Longrightarrow>
     static_flow_set V F e \<Longrightarrow>
     static_fan_in V e xC 
   "
